type soundness

TextbookTemplate.lean
@@ -289,3 +289,222 @@ theorem num_canonical :
   | inl => cases ty <;> contradiction
   | inr => assumption
 ```
+
+Now let's prove *syntactic type soundness*. Formally, syntactic type soundness
+says a well-typed term never gets stuck when evaluated under its small-step
+operational semantics. To establish syntactic type soundness, one typically
+proves two lemmas:
+
+* *Progress lemma*: A well-typed term is either a value or
+  it can take a step.
+* *Preservation lemma*: If a well-typed term can take a step,
+  the term it steps to is well-typed at the same
+  type.
+
+Let's prove each of these lemmas individually and then combine them
+to prove type syntactic type soundness.
+
+```savedLean
+theorem progress :
+  ∀ e : tm,
+  has_type e τ →
+  (value e) ∨ (∃ e', step e e') := by
+  intro e ty
+  induction ty with
+  | t_true =>
+    left
+    constructor
+    constructor
+  | t_false =>
+    left
+    constructor
+    constructor
+  | t_ite g thn els tyg tythn tyels =>
+    rename_i ih_g ih_thn ih_els
+    cases ih_g
+    · -- g is a value, use canonical forms to
+      -- extract it and take a step
+      rename_i val_g
+      obtain bool_g : bvalue g :=
+        by apply bool_canonical g tyg val_g
+      cases bool_g
+      · right
+        exists thn
+        constructor
+      · right
+        exists els
+        constructor
+    · -- g is not a value, it can step by IH
+      rename_i g_steps
+      right
+      obtain ⟨ g', g_steps ⟩ := g_steps
+      exists {{if [g'] then [thn] else [els]}}
+      apply step.st_if
+      assumption
+  | t_zro =>
+    left
+    right
+    constructor
+  | t_succ e' ty ih =>
+    cases ih
+    · -- e' is a value, use canonical forms lemma
+      rename_i val_e'
+      obtain num_e' : nvalue e' :=
+        by apply num_canonical e' ty val_e'
+      left
+      right
+      constructor
+      assumption
+    · -- e' is not a value, it can step by IH
+      rename_i e'_steps
+      right
+      obtain ⟨ e'', e''_steps ⟩ := e'_steps
+      exists {{ succ [e''] }}
+      constructor
+      assumption
+  | t_zero? e ty ih =>
+    cases ih
+    · -- e is a value
+      rename_i v
+      right
+      -- v is a value, step depending on if it's
+      -- 0 or succ v'
+      obtain num_v : nvalue e :=
+        by apply num_canonical e ty v
+      cases num_v
+      · -- step {{ zero? zero }} -> true
+        exists {{true}}
+        constructor
+      · -- step {{zero? (succ v)}} -> false
+        rename_i e' e'_v
+        exists {{false}}
+        constructor
+        assumption
+    · -- e is not a value; take a step
+      rename_i e' e_steps
+      right
+      obtain ⟨ e', e'_steps ⟩ := e_steps
+      exists {{ zero? [e'] }}
+      apply step.st_zero?
+      assumption
+  | t_pred e ty ih =>
+    cases ih
+    · -- e is a value. use canonical forms
+      rename_i v
+      obtain num_e : nvalue e :=
+        by apply num_canonical e ty v
+      cases num_e
+      · -- e = zero, pred zero -> zero
+        right
+        exists {{zero}}
+        apply step.st_pred0
+      · -- e = succ e', pred (succ e') -> e'
+        rename_i e' ty_e'
+        right
+        exists e'
+        apply step.st_pred_succ
+        assumption
+    · -- e is not a value, it can step by IH
+      rename_i e_steps
+      right
+      obtain ⟨ e', steps_e_e' ⟩ := e_steps
+      exists {{ pred [e'] }}
+      apply step.st_pred
+      assumption
+```
+
+```savedLean
+theorem preservation :
+  ∀ e : tm,
+  step e e' ->
+  has_type e τ ->
+  has_type e' τ := by
+  intro e step_e_e' ty
+  -- here we must use `generalizing`, since we want
+  -- e' to vary during induction and we've already
+  -- introduced it. We could accomplish the same
+  -- thing by using the `revert e'` tactic, which
+  -- moves `e'` back into the premise, but using
+  -- `generalizing` is cleaner.
+  induction ty generalizing e' with
+  | t_true => cases step_e_e'
+  | t_false => cases step_e_e'
+  | t_zro => cases step_e_e'
+  | t_ite g thn els tyg tythn tyels ihg ihthn ihels =>
+    cases step_e_e' with
+    | st_if_true | st_if_false => assumption
+    | st_if =>
+      rename_i g' step_g_g'
+      obtain g'_bool : has_type g' .Bool := by
+        apply ihg
+        assumption
+      apply has_type.t_ite
+      apply ihg
+      assumption
+      assumption
+      assumption
+  | t_succ e ty ih =>
+    cases step_e_e' with
+    | st_succ =>
+      rename_i e' step_e_e'
+      apply has_type.t_succ
+      apply ih
+      assumption
+  | t_pred e ty ih =>
+    cases step_e_e' with
+    | st_pred =>
+      rename_i e' step_e_e'
+      apply has_type.t_pred
+      apply ih
+      assumption
+    | st_pred0 =>
+      assumption
+    | st_pred_succ =>
+      cases ty
+      assumption
+  | t_zero? e ty ih =>
+    cases step_e_e' with
+    | st_zero? =>
+      rename_i e' step_e_e'
+      apply has_type.t_zero?
+      apply ih
+      assumption
+    | st_zero?_succ => constructor
+    | st_zero?_zero => constructor
+
+```
+
+```savedLean
+inductive multi {X : Type} (R : relation X) : relation X where
+  | multi_refl : ∀ (x : X), multi R x x
+  | multi_step : ∀ (x y z : X),
+                    R x y →
+                    multi R y z →
+                    multi R x z
+```
+
+```savedLean
+theorem syntactic_type_safety :
+  ∀ e : tm,
+  has_type e τ →
+  multi step e e' →
+  ¬ (stuck e') := by
+  intro e ty e_multi_e'
+  -- first apply preservation to show e' is well-typed
+  obtain ty_e' : has_type e' τ := by
+    induction e_multi_e' with
+    | multi_refl =>
+      assumption
+    | multi_step x y z x_step_y y_multistep_z ih =>
+      apply ih
+      apply preservation
+      assumption
+      assumption
+  intro ⟨ witness, contradiction ⟩
+  -- now apply preservation to show e' must take a step
+  -- or is a value, conclude by contradiction
+  obtain progr : (value e') ∨ (∃ e'', step e' e'')  := by
+    apply _root_.progress
+    assumption
+  cases progr <;> contradiction
+```
